Cleanup

src/Semantics/Equiv.dfy
@@ -27,6 +27,12 @@ module Bootstrap.Semantics.Equiv {
     type EqWV = Interp.EqWV // FIXME
     type Context = Values.Context
 
+    // TODO(SMH): move
+    predicate Seq_All<T>(f: T -> bool, s: seq<T>)
+    {
+      forall x | x in s :: f(x)
+    }
+
     // We introduce ``Equivs`` because in some situations we want to make ``EqValue``
     // and ``EqState`` opaque, and we can't (at least ``EqValue`` - see the comments for
     // this definition).
@@ -60,9 +66,9 @@ module Bootstrap.Semantics.Equiv {
 
     predicate GEqInterpResult<T(0)>(
       eq_ctx: (State,State) -> bool, eq_value: (T,T) -> bool, res: InterpResult<T>, res': InterpResult<T>)
-    // Interpretation results are equivalent.
-    // "G" stands for "generic".
-    // TODO: be a bit more precise in the error case, especially in case of "out of fuel".
+      // Interpretation results are equivalent.
+      // "G" stands for "generic".
+      // TODO(SMH): be a bit more precise in the error case, especially in case of "out of fuel".
     {
       match (res, res') {
         case (Success(Return(v,ctx)), Success(Return(v',ctx'))) =>
@@ -79,10 +85,10 @@ module Bootstrap.Semantics.Equiv {
       : (r: PureInterpResult<WV>)
       requires fn.Closure?
       requires |fn.vars| == |argvs|
-    // Small utility, very similar to ``InterpFunctionCall``, which we use to factorize
-    // the definitions. The opaque attribute is maybe not necessary anymore, but as the
-    // proofs work with it, we might as well keep it (it is easier to remove an opaque
-    // attribute, than to add one and fix the proofs by adding the proper calls to ``reveal``).
+      // Small utility, very similar to ``InterpFunctionCall``, which we use to factorize
+      // the definitions. The opaque attribute is maybe not necessary anymore, but as the
+      // proofs work with it, we might as well keep it (it is easier to remove an opaque
+      // attribute, than to add one and fix the proofs by adding the proper calls to ``reveal``).
     {
       var ctx := BuildCallState(fn.ctx, fn.vars, argvs);
       var Return(val, ctx) :- InterpExpr(fn.body, env, ctx);
@@ -91,26 +97,26 @@ module Bootstrap.Semantics.Equiv {
 
     predicate EqValue(v: WV, v': WV)
       decreases ValueTypeHeight(v) + ValueTypeHeight(v'), 1
-    // Equivalence between values.
-    //
-    // Two values are equivalent if:
-    // - they are not closures and are equal/have equivalent children values
-    // - they are closures and, when applied to equivalent inputs, they return equivalent outputs
-    //
-    // Rk.: we could write the predicate in a simpler manner by using `==` in case the values are not
-    // closures, but we prepare the terrain for a more general handling of collections.
-    //
-    // Rk.: for now, we assume the termination. This function terminates because the size of the
-    // type of the values decreases, the interesting case being the closures (see ``EqValue_Closure``).
-    // Whenever we find a closure `fn_ty = (ty_0, ..., ty_n) -> ret_ty`, we need to call ``EqValue``
-    // on valid inputs (with types `ty_i < fn_ty`) and on its output (with type `ret_ty < fn_ty`).
-    //
-    // Rk.: I initially wanted to make the definition opaque to prevent context saturation, because
-    // in most situations we don't need to know the content of EqValue.
-    // However it made me run into the following issue:
-    // BUG(https://github.com/dafny-lang/dafny/issues/2260)
-    // As ``EqValue`` appears a lot in foralls, using the `reveal` trick seemed too cumbersome
-    // to be a valid option.
+      // Equivalence between values.
+      //
+      // Two values are equivalent if:
+      // - they are not closures and are equal/have equivalent children values
+      // - they are closures and, when applied to equivalent inputs, they return equivalent outputs
+      //
+      // Rk.: we could write the predicate in a simpler manner by using `==` in case the values are not
+      // closures, but we prepare the terrain for a more general handling of collections.
+      //
+      // Rk.: for now, we assume the termination. This function terminates because the size of the
+      // type of the values decreases, the interesting case being the closures (see ``EqValue_Closure``).
+      // Whenever we find a closure `fn_ty = (ty_0, ..., ty_n) -> ret_ty`, we need to call ``EqValue``
+      // on valid inputs (with types `ty_i < fn_ty`) and on its output (with type `ret_ty < fn_ty`).
+      //
+      // Rk.: I initially wanted to make the definition opaque to prevent context saturation, because
+      // in most situations we don't need to know the content of EqValue.
+      // However it made me run into the following issue:
+      // BUG(https://github.com/dafny-lang/dafny/issues/2260)
+      // As ``EqValue`` appears a lot in foralls, using the `reveal` trick seemed too cumbersome
+      // to be a valid option.
     {
       match (v, v') {
         case (Unit, Unit) => true
@@ -160,11 +166,11 @@ module Bootstrap.Semantics.Equiv {
       requires v.Closure?
       requires v'.Closure?
       decreases ValueTypeHeight(v) + ValueTypeHeight(v'), 0
-    // Equivalence between values: closure case.
-    //
-    // See ``EqValue``.
-    //
-    // Rk.: contrary to ``EqValue``, it seems ok to make ``EqValue_Closure`` opaque.
+      // Equivalence between values: closure case.
+      //
+      // See ``EqValue``.
+      //
+      // Rk.: contrary to ``EqValue``, it seems ok to make ``EqValue_Closure`` opaque.
     {
       var Closure(ctx, vars, body) := v;
       var Closure(ctx', vars', body') := v';
@@ -215,35 +221,35 @@ module Bootstrap.Semantics.Equiv {
       GEqInterpResult(Mk_EqState(EqValue), eq_value, res, res')
     }
 
-    lemma EqValueHasEq_Lem(v: WV, v': WV)
+    lemma EqValueHasEq(v: WV, v': WV)
       requires EqValue(v,v')
       requires HasEqValue(v)
       requires HasEqValue(v')
       ensures v == v'
-    // If values are equivalent and have a decidable equality, they are necessarily equal.
+      // If values are equivalent and have a decidable equality, they are necessarily equal.
     {
       reveal EqValue_Closure();
     }
 
-    lemma EqValueHasEq_Forall_Lem()
+    lemma EqValueHasEq_Forall()
       ensures forall v: WV, v': WV | EqValue(v,v') && HasEqValue(v) && HasEqValue(v') :: v == v'
     {
       forall v: WV, v': WV | EqValue(v,v') && HasEqValue(v) && HasEqValue(v') ensures v == v' {
-        EqValueHasEq_Lem(v, v');
+        EqValueHasEq(v, v');
       }
     }
 
-    lemma EqInterp_Expr_EqState_Lem(e: Exprs.T, env: Environment, ctx: State, ctx': State)
+    lemma EqInterp_Expr_EqState(e: Exprs.T, env: Environment, ctx: State, ctx': State)
       requires SupportsInterp(e)
       requires EqState(ctx, ctx')
       ensures EqInterpResultValue(InterpExpr(e, env, ctx), InterpExpr(e, env, ctx'))
-    // The proof should be similar to ``EqInterp_Expr_CanBeMapLifted_Lem`` (and actually
-    // simpler), but I'm not sure how to efficiently factorize the two.
     {
+      // The proof should be similar to ``EqInterp_Expr_CanBeMapLifted`` (and actually
+      // simpler), but I'm not sure how to efficiently factorize the two.
       assume false; // TODO: prove
     }
 
-    lemma EqValue_Refl_Lem(v: WV)
+    lemma EqValue_Refl(v: WV)
       ensures EqValue(v, v)
       decreases v, 1
     {
@@ -258,24 +264,24 @@ module Bootstrap.Semantics.Equiv {
         case Map(m) => {
           ValueTypeHeight_Children_Lem(v); // For termination
           forall x | x in m ensures EqValue(m[x], m[x]) {
-            EqValue_Refl_Lem(m[x]);
+            EqValue_Refl(m[x]);
           }
         }
         case Multiset(ms) => {}
         case Seq(sq) => {
           ValueTypeHeight_Children_Lem(v); // For termination
           forall i | 0 <= i < |sq| ensures EqValue(sq[i], sq[i]) {
-            EqValue_Refl_Lem(sq[i]);
+            EqValue_Refl(sq[i]);
           }
         }
         case Set(st) => {}
         case Closure(ctx, vars, body) => {
-          EqValue_Closure_Refl_Lem(v);
+          EqValue_Closure_Refl(v);
         }
       }
     }
 
-    lemma BuildCallState_EqState_Lem(ctx: Context, ctx': Context, vars: seq<string>, argvs: seq<WV>, argvs': seq<WV>)
+    lemma BuildCallState_EqState(ctx: Context, ctx': Context, vars: seq<string>, argvs: seq<WV>, argvs': seq<WV>)
       requires WellFormedContext(ctx)
       requires WellFormedContext(ctx')
       requires |argvs| == |argvs'| == |vars|
@@ -286,7 +292,7 @@ module Bootstrap.Semantics.Equiv {
         var ctx1' := BuildCallState(ctx', vars, argvs');
         EqState(ctx1, ctx1')
     {
-      MapOfPairs_SeqZip_EqCtx_Lem(vars, argvs, argvs');
+      MapOfPairs_SeqZip_EqCtx(vars, argvs, argvs');
       var m := MapOfPairs(Seq.Zip(vars, argvs));
       var m' := MapOfPairs(Seq.Zip(vars, argvs'));
       reveal BuildCallState();
@@ -297,7 +303,7 @@ module Bootstrap.Semantics.Equiv {
       assert ctx1'.locals == ctx' + m';
     }
 
-    lemma EqValue_Closure_Refl_Lem(v: WV)
+    lemma EqValue_Closure_Refl(v: WV)
       requires v.Closure?
       ensures EqValue_Closure(v, v)
       decreases v, 0
@@ -320,35 +326,35 @@ module Bootstrap.Semantics.Equiv {
           var res' := InterpCallFunctionBody(v, env, argvs');
 
           assert EqCtx(ctx, ctx) by {
-            // It would be difficult to call a lemma like ``EqState_Refl_Lem`` here, because
+            // It would be difficult to call a lemma like ``EqState_Refl`` here, because
             // of termination issues. However, we have that the values in the closure context
             // are smaller than the closure value itself, which allows us to recursively call
             // ``EqValue``.
             forall x | x in ctx ensures EqValue(ctx[x], ctx[x]) {
-              EqValue_Refl_Lem(ctx[x]);
+              EqValue_Refl(ctx[x]);
             }
             reveal GEqCtx();
           }
 
           var ctx1 := BuildCallState(ctx, vars, argvs);
           var ctx1' := BuildCallState(ctx, vars, argvs');
-          BuildCallState_EqState_Lem(ctx, ctx, vars, argvs, argvs');
+          BuildCallState_EqState(ctx, ctx, vars, argvs, argvs');
           assert EqState(ctx1, ctx1');
 
           reveal InterpCallFunctionBody();
-          EqInterp_Expr_EqState_Lem(body, env, ctx1, ctx1');
+          EqInterp_Expr_EqState(body, env, ctx1, ctx1');
           assert EqPureInterpResultValue(res, res');
       }
     }
 
-    lemma EqState_Refl_Lem(ctx: State)
+    lemma EqState_Refl(ctx: State)
       ensures EqState(ctx, ctx)
     {
       reveal GEqCtx();
-      EqValue_Refl_Forall_Lem();
+      EqValue_Refl_Forall();
     }
 
-    lemma EqValue_Trans_Lem(v0: WV, v1: WV, v2: WV)
+    lemma EqValue_Trans(v0: WV, v1: WV, v2: WV)
       requires EqValue(v0, v1)
       requires EqValue(v1, v2)
       ensures EqValue(v0, v2)
@@ -365,21 +371,21 @@ module Bootstrap.Semantics.Equiv {
         case Map(m0) =>
           ValueTypeHeight_Children_Lem(v0); // For termination
           forall x | x in m0 ensures EqValue(v0.m[x], v2.m[x]) {
-            EqValue_Trans_Lem(v0.m[x], v1.m[x], v2.m[x]);
+            EqValue_Trans(v0.m[x], v1.m[x], v2.m[x]);
           }
         case Multiset(ms) => {}
         case Seq(sq) =>
           ValueTypeHeight_Children_Lem(v0); // For termination
           forall i | 0 <= i < |sq| ensures EqValue(v0.sq[i], v2.sq[i]) {
-            EqValue_Trans_Lem(v0.sq[i], v1.sq[i], v2.sq[i]);
+            EqValue_Trans(v0.sq[i], v1.sq[i], v2.sq[i]);
           }
         case Set(st) => {}
         case Closure(ctx, vars, body) =>
-          EqValue_Closure_Trans_Lem(v0, v1, v2);
+          EqValue_Closure_Trans(v0, v1, v2);
       }
     }
 
-    lemma EqValue_Closure_Trans_Lem(v0: WV, v1: WV, v2: WV)
+    lemma EqValue_Closure_Trans(v0: WV, v1: WV, v2: WV)
       requires v0.Closure?
       requires v1.Closure?
       requires v2.Closure?
@@ -416,7 +422,7 @@ module Bootstrap.Semantics.Equiv {
           assume (forall i | 0 <= i < |vars0| :: ValueTypeHeight(argvs0[i]) < ValueTypeHeight(v1));
 
           forall i | 0 <= i < |vars0| ensures EqValue(argvs0[i], argvs0[i]) {
-            EqValue_Refl_Lem(argvs0[i]);
+            EqValue_Refl(argvs0[i]);
           }
 
           var res1 := InterpCallFunctionBody(v1, env, argvs0);
@@ -429,7 +435,7 @@ module Bootstrap.Semantics.Equiv {
             // trivially true.
             assume ValueTypeHeight(ov0) < ValueTypeHeight(v0);
 
-            EqValue_Trans_Lem(ov0, ov1, ov2);
+            EqValue_Trans(ov0, ov1, ov2);
 
             assert EqPureInterpResultValue(res0, res2);
           }
@@ -440,70 +446,70 @@ module Bootstrap.Semantics.Equiv {
       }
     }
 
-    lemma {:induction v, v'} EqValue_HasEqValue_Lem(v: WV, v': WV)
+    lemma {:induction v, v'} EqValue_HasEqValue(v: WV, v': WV)
       requires EqValue(v, v')
       ensures HasEqValue(v) == HasEqValue(v')
     {}
 
-    lemma EqValue_HasEqValue_Forall_Lem()
+    lemma EqValue_HasEqValue_Forall()
       ensures forall v: WV, v': WV | EqValue(v, v') :: HasEqValue(v) == HasEqValue(v')
     {
       forall v: WV, v': WV | EqValue(v, v') ensures HasEqValue(v) == HasEqValue(v') {
-        EqValue_HasEqValue_Lem(v, v');
+        EqValue_HasEqValue(v, v');
       }
     }
 
-    lemma EqValue_HasEqValue_Eq_Lem(v: WV, v': WV)
+    lemma EqValue_HasEqValue_Eq(v: WV, v': WV)
       requires EqValue(v, v')
       ensures HasEqValue(v) == HasEqValue(v')
       ensures HasEqValue(v) ==> v == v'
     {
-      EqValue_HasEqValue_Lem(v, v');
+      EqValue_HasEqValue(v, v');
       if HasEqValue(v) || HasEqValue(v') {
-        EqValueHasEq_Lem(v, v');
+        EqValueHasEq(v, v');
       }
     }
 
-    lemma EqValue_HasEqValue_Eq_Forall_Lem()
+    lemma EqValue_HasEqValue_Eq_Forall()
       ensures forall v:WV, v':WV | EqValue(v, v') ::
         && (HasEqValue(v) == HasEqValue(v'))
         && (HasEqValue(v) ==> v == v')
-    // This is one of the important lemmas for the proofs of equivalence.
-    // The reason is that the interpreter often checks that some values
-    // have a decidable equality (for instance, before inserting a value in
-    // a set). When doing equivalence proofs, for instance to prove that the
-    // same instruction evaluated in equivalent contexts generates equivalent
-    // results, we often want:
-    // - to know that the check succeeds in both cases, or fails in both cases
-    // - to know that if it succeeded, then the valuevs are equal
+      // This is one of the important lemmas for the proofs of equivalence.
+      // The reason is that the interpreter often checks that some values
+      // have a decidable equality (for instance, before inserting a value in
+      // a set). When doing equivalence proofs, for instance to prove that the
+      // same instruction evaluated in equivalent contexts generates equivalent
+      // results, we often want:
+      // - to know that the check succeeds in both cases, or fails in both cases
+      // - to know that if it succeeded, then the valuevs are equal
     {
       forall v:WV, v':WV | EqValue(v, v')
         ensures
         && (HasEqValue(v) == HasEqValue(v'))
         && (HasEqValue(v) ==> v == v') {
-          EqValue_HasEqValue_Eq_Lem(v, v');
+          EqValue_HasEqValue_Eq(v, v');
       }
     }
 
-    lemma EqValue_Refl_Forall_Lem()
+    lemma EqValue_Refl_Forall()
       ensures forall v : WV :: EqValue(v, v)
     {
       forall v : WV | true
         ensures EqValue(v, v)
       {
-        EqValue_Refl_Lem(v);
+        EqValue_Refl(v);
         assert EqValue(v, v);
       }
     }
 
-    lemma EqState_Trans_Lem(ctx0: State, ctx1: State, ctx2: State)
+    lemma EqState_Trans(ctx0: State, ctx1: State, ctx2: State)
       requires EqState(ctx0, ctx1)
       requires EqState(ctx1, ctx2)
       ensures EqState(ctx0, ctx2)
     {
       reveal GEqCtx();
       forall x | x in ctx0.locals.Keys ensures EqValue(ctx0.locals[x], ctx2.locals[x]) {
-        EqValue_Trans_Lem(ctx0.locals[x], ctx1.locals[x], ctx2.locals[x]);
+        EqValue_Trans(ctx0.locals[x], ctx1.locals[x], ctx2.locals[x]);
       }
     }
 
@@ -550,15 +556,18 @@ module Bootstrap.Semantics.Equiv {
       EqInterpResult(EqValue, res, res')
     }
 
-    predicate EqInterpResultSeqValue(res: InterpResult<seq<WV>>, res': InterpResult<seq<WV>>) {
+    predicate EqInterpResultSeqValue(res: InterpResult<seq<WV>>, res': InterpResult<seq<WV>>)
+    {
       EqInterpResult(EqSeqValue, res, res')
     }
 
-    predicate GEqInterpResultSeq(eq: Equivs, res: InterpResult<seq<WV>>, res': InterpResult<seq<WV>>) {
+    predicate GEqInterpResultSeq(eq: Equivs, res: InterpResult<seq<WV>>, res': InterpResult<seq<WV>>)
+    {
       GEqInterpResult(eq.eq_state, (x, x') => EqSeq(eq.eq_value, x, x'), res, res')
     }
 
-    predicate EqPureInterpResult<T(0)>(eq_values: (T,T) -> bool, res: PureInterpResult<T>, res': PureInterpResult<T>) {
+    predicate EqPureInterpResult<T(0)>(eq_values: (T,T) -> bool, res: PureInterpResult<T>, res': PureInterpResult<T>)
+    {
       match (res, res') {
         case (Success(v), Success(v')) =>
           eq_values(v, v')
@@ -569,15 +578,18 @@ module Bootstrap.Semantics.Equiv {
       }
     }
 
-    predicate EqPureInterpResultValue(res: PureInterpResult<WV>, res': PureInterpResult<WV>) {
+    predicate EqPureInterpResultValue(res: PureInterpResult<WV>, res': PureInterpResult<WV>)
+    {
       EqPureInterpResult(EqValue, res, res')
     }
 
-    predicate EqPureInterpResultSeqValue(res: PureInterpResult<seq<WV>>, res': PureInterpResult<seq<WV>>) {
+    predicate EqPureInterpResultSeqValue(res: PureInterpResult<seq<WV>>, res': PureInterpResult<seq<WV>>)
+    {
       EqPureInterpResult(EqSeqValue, res, res')
     }
 
-    predicate EqInterpResultSeq1Value(res: InterpResult<WV>, res': InterpResult<seq<WV>>) {
+    predicate EqInterpResultSeq1Value(res: InterpResult<WV>, res': InterpResult<seq<WV>>)
+    {
       match (res, res') {
         case (Success(Return(v,ctx)), Success(Return(sv,ctx'))) =>
           && |sv| == 1
@@ -590,7 +602,25 @@ module Bootstrap.Semantics.Equiv {
       }
     }
 
-    predicate EqInterpResultSeq1Value_Strong(res: InterpResult<WV>, res': InterpResult<seq<WV>>) {
+    predicate EqInterpResultValue_Strong(res: InterpResult<WV>, res': InterpResult<WV>)
+      // Equality predicate about results, using a *strong* equality rather than our weak
+      // notion of equivalence.
+    {
+      match (res, res') {
+        case (Success(Return(v,ctx)), Success(Return(v',ctx'))) =>
+          && v == v'
+          && ctx == ctx'
+        case (Failure(err), Failure(err')) =>
+          err == err'
+        case _ =>
+          false
+      }
+    }
+
+    predicate EqInterpResultSeq1Value_Strong(res: InterpResult<WV>, res': InterpResult<seq<WV>>)
+      // Equality predicate about results, using a *strong* equality rather than our weak
+      // notion of equivalence.
+    {
       match (res, res') {
         case (Success(Return(v,ctx)), Success(Return(sv,ctx'))) =>
           && sv == [v]
@@ -604,7 +634,7 @@ module Bootstrap.Semantics.Equiv {
 
     // TODO: make opaque?
     predicate GEqInterp(eq: Equivs, e: Exprs.T, e': Exprs.T)
-    // This is the important, generic equivalence relation over expressions.
+      // This is the important, generic equivalence relation over expressions.
     {
       SupportsInterp(e) ==>
       (&& SupportsInterp(e')
@@ -618,14 +648,25 @@ module Bootstrap.Semantics.Equiv {
       (e, e') => GEqInterp(eq, e, e')
     }
 
-    // TODO: make opaque?
+    // TODO(SMH): make opaque?
     predicate EqInterp(e: Exprs.T, e': Exprs.T)
-    // The important equivalence relation over expressions.
+      // The important equivalence relation over expressions.
     {
       GEqInterp(EQ(EqValue, Mk_EqState(EqValue)), e, e')
     }
 
-    lemma EqInterp_Refl_Lem(e: Exprs.T)
+    // TODO(SMH): make opaque?
+    predicate EqInterpBlockExprs(es: seq<Exprs.T>, es': seq<Exprs.T>)
+    {
+      Seq_All(SupportsInterp, es) ==>
+      (&& Seq_All(SupportsInterp, es')
+       && forall env, ctx, ctx' | EqState(ctx, ctx') ::
+         EqInterpResultValue(
+                        InterpBlock_Exprs(es, env, ctx),
+                        InterpBlock_Exprs(es', env, ctx')))
+    }
+
+    lemma EqInterp_Refl(e: Exprs.T)
       ensures EqInterp(e, e)
     {
       if SupportsInterp(e) {
@@ -635,10 +676,17 @@ module Bootstrap.Semantics.Equiv {
                          InterpExpr(e, env, ctx),
                          InterpExpr(e, env, ctx'))
         {
-          EqInterp_Expr_EqState_Lem(e, env, ctx, ctx');
+          EqInterp_Expr_EqState(e, env, ctx, ctx');
         }
       }
     }
+
+    lemma EqInterpBlockExprs_Inst(es: seq<Exprs.T>, es': seq<Exprs.T>, env: Environment, ctx: State, ctx': State)
+      requires EqInterpBlockExprs(es, es')
+      requires Seq_All(SupportsInterp, es)
+      requires EqState(ctx, ctx')
+      ensures  EqInterpResultValue(InterpBlock_Exprs(es, env, ctx), InterpBlock_Exprs(es', env, ctx'))
+    {}
 
     predicate All_Rel_Forall<A, B>(rel: (A,B) -> bool, xs: seq<A>, ys: seq<B>)
     {
@@ -646,15 +694,15 @@ module Bootstrap.Semantics.Equiv {
       && forall i | 0 <= i < |xs| :: rel(xs[i], ys[i])
     }
 
-    lemma EqInterp_Seq_Refl_Lem(es: seq<Exprs.T>)
+    lemma EqInterp_Seq_Refl(es: seq<Exprs.T>)
       ensures All_Rel_Forall(EqInterp, es, es)
     {
       forall i | 0 <= i < |es| ensures EqInterp(es[i], es[i]) {
-        EqInterp_Refl_Lem(es[i]);
+        EqInterp_Refl(es[i]);
       }
     }
 
-    lemma EqInterp_Trans_Lem(e0: Exprs.T, e1: Exprs.T, e2: Exprs.T)
+    lemma EqInterp_Trans(e0: Exprs.T, e1: Exprs.T, e2: Exprs.T)
       requires EqInterp(e0, e1)
       requires EqInterp(e1, e2)
       ensures EqInterp(e0, e2)
@@ -663,7 +711,7 @@ module Bootstrap.Semantics.Equiv {
         forall env, ctx, ctx' | EqState(ctx, ctx')
           ensures EqInterpResultValue(InterpExpr(e0, env, ctx), InterpExpr(e2, env, ctx'))
         {
-          EqState_Refl_Lem(ctx);
+          EqState_Refl(ctx);
           assert EqState(ctx, ctx);
           var res0 := InterpExpr(e0, env, ctx);
           var res1 := InterpExpr(e1, env, ctx);
@@ -672,8 +720,8 @@ module Bootstrap.Semantics.Equiv {
           assert EqInterpResultValue(res1, res2);
 
           if res0.Success? {
-            EqValue_Trans_Lem(res0.value.ret, res1.value.ret, res2.value.ret);
-            EqState_Trans_Lem(res0.value.ctx, res1.value.ctx, res2.value.ctx);
+            EqValue_Trans(res0.value.ret, res1.value.ret, res2.value.ret);
+            EqState_Trans(res0.value.ctx, res1.value.ctx, res2.value.ctx);
           }
           else {}
         }
@@ -685,16 +733,15 @@ module Bootstrap.Semantics.Equiv {
       forall x0, x1, x2 | rel(x0, x1) && rel(x1, x2) :: rel(x0, x2)
     }
 
-    lemma EqInterp_IsTransitive_Lem()
+    lemma EqInterp_IsTransitive()
       ensures RelIsTransitive(EqInterp)
     {
       forall e0, e1, e2 | EqInterp(e0, e1) && EqInterp(e1, e2) ensures EqInterp(e0, e2) {
-        EqInterp_Trans_Lem(e0, e1, e2);
+        EqInterp_Trans(e0, e1, e2);
       }
     }
 
-    // TODO(SHM): rename to ``InterpExprs1_Strong_Eq``
-    lemma InterpExprs1_Strong_Lem(e: Expr, env: Environment, ctx: State)
+    lemma InterpExprs1_Strong_Eq(e: Expr, env: Environment, ctx: State)
       requires SupportsInterp(e)
       ensures forall e' | e' in [e] :: SupportsInterp(e')
       ensures EqInterpResultSeq1Value_Strong(InterpExpr(e, env, ctx), InterpExprs([e], env, ctx))
@@ -720,7 +767,34 @@ module Bootstrap.Semantics.Equiv {
       }
     }
 
-    lemma EqInterp_Lem(e: Exprs.T, e': Exprs.T, env: Environment, ctx: State, ctx': State)
+    lemma InterpBlock_Exprs_Refl(es: seq<Expr>, env: Environment, ctx: State, ctx': State)
+      requires Seq_All(SupportsInterp, es)
+      requires EqState(ctx, ctx')
+      ensures EqInterpResultValue(InterpBlock_Exprs(es, env, ctx), InterpBlock_Exprs(es, env, ctx'))
+    {
+      reveal InterpBlock_Exprs();
+      if es == [] {}
+      else {
+         // Evaluate the first expression
+        var res0 := InterpExpr(es[0], env, ctx);
+        var res0' := InterpExpr(es[0], env, ctx');
+        EqInterp_Refl(es[0]);
+        EqInterp_Inst(es[0], es[0], env, ctx, ctx');
+
+        // Evaluate the remaining expressions
+        if res0.Success? && res0.value.ret == V.Unit {
+          var Return(_, ctx0) := res0.value;
+          var Return(_, ctx0') := res0'.value;
+
+          InterpBlock_Exprs_Refl(es[1..], env, ctx0, ctx0');
+        }
+        else {
+          // Trivial
+        }
+      }
+    }
+
+    lemma EqInterp_Inst(e: Exprs.T, e': Exprs.T, env: Environment, ctx: State, ctx': State)
       requires SupportsInterp(e)
       requires EqInterp(e, e')
       requires EqState(ctx, ctx')
@@ -729,7 +803,7 @@ module Bootstrap.Semantics.Equiv {
     // We use this lemma because sometimes quantifiers are are not triggered.
     {}
 
-    lemma InterpExprs_GEqInterp_Lem(
+    lemma InterpExprs_GEqInterp_Inst(
       eq: Equivs, es: seq<Expr>, es': seq<Expr>, env: Environment, ctx: State, ctx': State)
       requires forall e | e in es :: SupportsInterp(e)
       requires All_Rel_Forall(Mk_EqInterp(eq), es, es')
@@ -771,7 +845,7 @@ module Bootstrap.Semantics.Equiv {
             var res2' := InterpExprs(es'[1..], env, ctx1');
 
             // Recursive call
-            InterpExprs_GEqInterp_Lem(eq, es[1..], es'[1..], env, ctx1, ctx1');
+            InterpExprs_GEqInterp_Inst(eq, es[1..], es'[1..], env, ctx1, ctx1');
 
             match res2 {
               case Success(Return(vs, ctx2)) => {
@@ -792,7 +866,7 @@ module Bootstrap.Semantics.Equiv {
       }
     }
 
-    lemma InterpExprs_EqInterp_Lem(es: seq<Expr>, es': seq<Expr>, env: Environment, ctx: State, ctx': State)
+    lemma InterpExprs_EqInterp_Inst(es: seq<Expr>, es': seq<Expr>, env: Environment, ctx: State, ctx': State)
       requires forall e | e in es :: SupportsInterp(e)
       requires All_Rel_Forall(EqInterp, es, es')
       requires EqState(ctx, ctx')
@@ -801,10 +875,10 @@ module Bootstrap.Semantics.Equiv {
     // Auxiliary lemma: if two sequences contain equivalent expressions, evaluating those two
     // sequences in equivalent contexts leads to equivalent results.
     {
-      InterpExprs_GEqInterp_Lem(EQ(EqValue, EqState), es, es', env, ctx, ctx');
+      InterpExprs_GEqInterp_Inst(EQ(EqValue, EqState), es, es', env, ctx, ctx');
     }
 
-    lemma Map_PairOfMapDisplaySeq_Lem(e: Interp.Expr, e': Interp.Expr, argvs: seq<WV>, argvs': seq<WV>)
+    lemma Map_PairOfMapDisplaySeq(e: Interp.Expr, e': Interp.Expr, argvs: seq<WV>, argvs': seq<WV>)
       requires EqSeqValue(argvs, argvs')
       ensures EqPureInterpResult(EqSeqPairEqValueValue,
                                  Seq.MapResult(argvs, argv => PairOfMapDisplaySeq(e, argv)),
@@ -820,13 +894,13 @@ module Bootstrap.Semantics.Equiv {
         var res0 := PairOfMapDisplaySeq(e, argv);
         var res0' := PairOfMapDisplaySeq(e', argv');
 
-        EqValue_HasEqValue_Eq_Forall_Lem();
+        EqValue_HasEqValue_Eq_Forall();
         if res0.Success? {
           assert res0'.Success?;
           assert EqPureInterpResult(EqPairEqValueValue, res0, res0');
 
           reveal Seq.MapResult();
-          Map_PairOfMapDisplaySeq_Lem(e, e', argvs[1..], argvs'[1..]);
+          Map_PairOfMapDisplaySeq(e, e', argvs[1..], argvs'[1..]);
         }
         else {
           // Trivial
@@ -834,32 +908,32 @@ module Bootstrap.Semantics.Equiv {
       }
     }
 
-    lemma MapOfPairs_EqArgs_Lem(argvs: seq<(EqWV, WV)>, argvs': seq<(EqWV, WV)>)
+    lemma MapOfPairs_EqArgs(argvs: seq<(EqWV, WV)>, argvs': seq<(EqWV, WV)>)
       requires EqSeqPairEqValueValue(argvs, argvs')
       ensures EqMap(EqValue, MapOfPairs(argvs), MapOfPairs(argvs'))
     {
       if argvs == [] {}
       else {
         var lastidx := |argvs| - 1;
-        EqValueHasEq_Forall_Lem();
-        MapOfPairs_EqArgs_Lem(argvs[..lastidx], argvs'[..lastidx]);
+        EqValueHasEq_Forall();
+        MapOfPairs_EqArgs(argvs[..lastidx], argvs'[..lastidx]);
       }
     }
 
-    lemma InterpMapDisplay_EqArgs_Lem(e: Interp.Expr, e': Interp.Expr, argvs: seq<WV>, argvs': seq<WV>)
+    lemma InterpMapDisplay_EqArgs(e: Interp.Expr, e': Interp.Expr, argvs: seq<WV>, argvs': seq<WV>)
       requires EqSeqValue(argvs, argvs')
       ensures EqPureInterpResult(EqMapValue, InterpMapDisplay(e, argvs), InterpMapDisplay(e', argvs')) {
       var res0 := Seq.MapResult(argvs, argv => PairOfMapDisplaySeq(e, argv));
       var res0' := Seq.MapResult(argvs', argv => PairOfMapDisplaySeq(e', argv));
 
-      Map_PairOfMapDisplaySeq_Lem(e, e', argvs, argvs');
-      EqValue_HasEqValue_Eq_Forall_Lem();
+      Map_PairOfMapDisplaySeq(e, e', argvs, argvs');
+      EqValue_HasEqValue_Eq_Forall();
 
       match res0 {
         case Success(pairs) => {
           var pairs' := res0'.value;
 
-          MapOfPairs_EqArgs_Lem(pairs, pairs');
+          MapOfPairs_EqArgs(pairs, pairs');
 
           var m := MapOfPairs(pairs);
           var m' := MapOfPairs(pairs');
@@ -871,7 +945,7 @@ module Bootstrap.Semantics.Equiv {
       }
     }
 
-    lemma MapOfPairs_EqCtx_Lem(pl: seq<(string, WV)>, pl': seq<(string, WV)>)
+    lemma MapOfPairs_EqCtx(pl: seq<(string, WV)>, pl': seq<(string, WV)>)
       requires |pl| == |pl'|
       requires (forall i | 0 <= i < |pl| :: pl[i].0 == pl'[i].0)
       requires (forall i | 0 <= i < |pl| :: EqValue(pl[i].1, pl'[i].1))
@@ -884,14 +958,14 @@ module Bootstrap.Semantics.Equiv {
       if pl == [] {}
       else {
         var lastidx := |pl| - 1;
-        MapOfPairs_EqCtx_Lem(pl[..lastidx], pl'[..lastidx]);
+        MapOfPairs_EqCtx(pl[..lastidx], pl'[..lastidx]);
       }
     }
 
     // (SMH) I don't understand why I need to use vcs_split_on_every_assert on this one.
     // For some strange reason it takes ~20s to verify with this, and timeouts without.
     lemma {:vcs_split_on_every_assert}
-    MapOfPairs_SeqZip_EqCtx_Lem(vars: seq<string>, argvs: seq<WV>, argvs': seq<WV>)
+    MapOfPairs_SeqZip_EqCtx(vars: seq<string>, argvs: seq<WV>, argvs': seq<WV>)
       requires |argvs| == |argvs'| == |vars|
       requires (forall i | 0 <= i < |vars| :: EqValue(argvs[i], argvs'[i]))
       ensures
@@ -907,6 +981,77 @@ module Bootstrap.Semantics.Equiv {
       assert forall i | 0 <= i < |pl| :: EqValue(pl[i].1, pl'[i].1);
 
       reveal GEqCtx();
-      MapOfPairs_EqCtx_Lem(pl, pl');
+      MapOfPairs_EqCtx(pl, pl');
+    }
+
+    lemma InterpBlock_Exprs_Eq_Append(e: Expr, e': Expr, tl: seq<Expr>, tl': seq<Expr>, env: Environment, ctx: State, ctx': State)
+      requires SupportsInterp(e)
+      requires SupportsInterp(e')
+      requires Seq_All(SupportsInterp, tl)
+      requires Seq_All(SupportsInterp, tl')
+      requires EqState(ctx, ctx')
+      requires EqInterp(e, e')
+      requires EqInterpBlockExprs(tl, tl')
+      requires |tl| > 0
+      ensures EqInterpResultValue(InterpBlock_Exprs([e] + tl, env, ctx), InterpBlock_Exprs([e'] + tl', env, ctx'))
+      // Auxiliary lemma for the proofs about transformations operating on blocks. This is especially
+      // useful when those transformations might update the length of the sequence of expressions
+      // in the blocks. The proof is a bit tricky, because the case where the sequence has length 1
+      // is a special case in the definition of ``EqInterpBlock_Exprs``.
+    {
+      var es := [e] + tl;
+      var es' := [e'] + tl';
+      assert e == es[0];
+
+      reveal InterpBlock_Exprs();
+
+      // Evaluate the first expression
+      var res0 := InterpExpr(e, env, ctx);
+      var res0' := InterpExpr(e', env, ctx');
+      EqInterp_Inst(e, e', env, ctx, ctx');
+
+      // We need to make a case disjunction on whether the length of the concatenated sequences is
+      // > 1 or not
+      if |tl'| >= 1 {
+        // The "regular" case
+
+        // Evaluate the remaining expressions
+        if res0.Success? && res0.value.ret == V.Unit {
+          var Return(_, ctx0) := res0.value;
+          var Return(_, ctx0') := res0'.value;
+
+          var res1 := InterpBlock_Exprs(tl, env, ctx0);
+          var res1' := InterpBlock_Exprs(tl', env, ctx0');
+
+          EqInterpBlockExprs_Inst(tl, tl', env, ctx0, ctx0');
+        }
+        else {
+          // Trivial
+        }
+      }
+      else {
+        // Degenerate case
+        assert |tl'| == 0;
+
+        if res0.Success? {
+          var Return(v, ctx0) := res0.value;
+          var Return(v', ctx0') := res0'.value;
+
+          if v == V.Unit {
+            assert v' == V.Unit;
+            EqInterpBlockExprs_Inst(tl, tl', env, ctx0, ctx0');
+          }
+          else {
+            assert v' != V.Unit;
+
+            // TODO(SMH): update EqInterp so that this works (evaluating `es` will fail if `e` doesn't
+            // evaluate to `Unit`)
+            assume false; // TODO: prove
+          }
+        }
+        else {
+          // Trivial
+        }
+      }
     }
 }
